change local heap to global heap

theories/Crypt/package/pkg_rhl.v
@@ -35,6 +35,7 @@ Module PackageRHL (π : RulesParam).
 
   Import π.
   Include (PackageNotation π).
+  Include (DerivedRules π).
 
   Local Open Scope fset.
   Local Open Scope fset_scope.
@@ -55,44 +56,25 @@ Module PackageRHL (π : RulesParam).
     Definition Adversary4Game (Game_export : Interface) : Type :=
       package Game_export A_export.
 
-
     Open Scope fset.
-    Let iops_StP := @ops_StP probE rel_choiceTypes chEmb.
-    Let iar_StP := @ar_StP probE rel_choiceTypes chEmb.
+    (* Let iops_StP := @ops_StP probE rel_choiceTypes chEmb. *)
+    (* Let iar_StP := @ar_StP probE rel_choiceTypes chEmb. *)
 
-    Definition dommHeap (s : {fset Location}) := { x : Location | x \in s }.
-
-    Definition makeHeap (s : {fset Location}) :=
-      {fmap (dommHeap s) → Value}.
-
-    Definition makeHeap_cT (s : {fset Location}) :=
-      [choiceType of (makeHeap s)].
+    Definition heap := {fmap Location -> Value}.
+    Definition heap_choiceType := [choiceType of heap].
 
     Definition Game_op_import_S : Type := {_ : ident & void}.
     Definition Game_import_P : Game_op_import_S → choiceType :=
       fun v => match v with existT a b => match b with end end.
 
-    Definition getFromMap
-               {locs : {fset Location}}
-               (map : {fmap {x : Location | x \in locs} → Value})
-               (l : Location) (H : l \in locs) : Value.
+    Definition get_heap (map : heap) (l : Location) : Value.
     Proof.
-      destruct (getm map (exist _ l H)) eqn:Hget.
+      destruct (getm map l).
       + exact s.
       + exact 0.
     Defined.
 
-    Arguments getFromMap {_} _ _ {_}.
-
-    Definition setFromMap
-               {locs : {fset Location}}
-               (map : {fmap {x : Location | x \in locs} → Value})
-               (l : Location) (H : l \in locs) (v : Value) : {fmap {x : Location | x \in locs} → Value}.
-    Proof.
-      apply (setm map).
-      - exists l. exact H.
-      - exact v.
-    Defined.
+    Definition set_heap (map : heap) (l : Location)  (v : Value) : heap := setm map l v.
 
     Definition fromEmpty {B} {v : opsig} (H : v \in fset0) : B.
       rewrite in_fset0 in H.
@@ -123,28 +105,83 @@ Module PackageRHL (π : RulesParam).
 
     Set Equations Transparent.
 
-    Equations? FreeTranslate' {B : choiceType} {locs : {fset Location}}
-      (p : raw_program B) (h : valid_program locs Game_import p)
-    : rFreeF (iops_StP (makeHeap_cT locs)) (iar_StP (makeHeap_cT locs)) B :=
-      FreeTranslate' p h with p := {
+    Equations? repr' {B : choiceType} {L : {fset Location}}
+      (p : raw_program B) (h : valid_program L Game_import p)
+    : rFreeF (ops_StP heap_choiceType) (ar_StP heap_choiceType) B :=
+      repr' p h with p := {
       | _ret x := retrFree _ ;
       | _opr o x k := False_rect _ _ ;
-      | _getr l k := ropr (inl (inl (gett _))) (λ s, let v := getFromMap s l in FreeTranslate' (k v) _) ;
+      | _getr l k := ropr (inl (inl (gett _))) (λ s, let v := get_heap s l in repr' (k v) _) ;
       | _putr l v k :=
-        ropr (inl (inl (gett (makeHeap_cT locs)))) (λ s, ropr (inl (inr (putt (makeHeap_cT locs) (setFromMap s l _ v)))) (λ s', FreeTranslate' k _)) ;
-      | _sampler op k := ropr (inr op) (λ s, FreeTranslate' (k s) _)
+        ropr (inl (inl (gett heap_choiceType))) (λ s, ropr (inl (inr (putt heap_choiceType (set_heap s l v)))) (λ s', repr' k _)) ;
+      | _sampler op k := ropr (inr op) (λ s, repr' (k s) _)
       }.
     Proof.
       - destruct h as [hin _]. eapply fromEmpty. exact hin.
       - cbn in h. intuition auto.
       - cbn in h. destruct h as [ho h]. apply h.
-      - cbn in h. intuition auto.
-      - cbn in h. destruct h as [ho h]. apply h.
     Defined.
 
-    Definition FreeTranslate {B locs} (p : program locs Game_import B) :=
+    Definition repr {B locs} (p : program locs Game_import B) :=
       let '(exist p h) := p in
-      FreeTranslate' p h.
+      repr' p h.
+
+    Ltac fold_repr :=
+      change (repr' ?p ?h) with (repr (exist _ p h)).
+
+    Lemma repr'_ext {B L1 L2} (p1 p2 : raw_program B)
+          (hp1 : valid_program L1 Game_import p1) (hp2 : valid_program L2 Game_import p2)
+          (H : p1 = p2)
+      : repr' p1 hp1 = repr' p2 hp2.
+    Proof.
+      destruct H.
+      induction p1.
+      - cbn. reflexivity.
+      - pose f := hp1. destruct f as [hin _].
+        eapply fromEmpty. exact hin.
+      - cbn in hp1, hp2.
+        cbn. f_equal. extensionality s.
+        apply H.
+      - cbn. f_equal. extensionality s.
+        f_equal. extensionality s'.
+        apply IHp1.
+      - cbn. f_equal. extensionality s.
+        apply H.
+    Qed.
+
+    Lemma repr_bind {B C} {L}
+          (p : program L Game_import B) (f : B -> program L Game_import C) :
+      repr (bind _ _ p f) =  bindrFree _ _ (repr p) (fun b => repr (f b)).
+    Proof.
+      destruct p as [p h].
+      induction p.
+      - cbn. fold_repr.
+        f_equal.
+        apply program_ext.
+        simpl. reflexivity.
+      - cbn in h. destruct h as [h1 h2]. eapply fromEmpty. exact h1.
+      - cbn. f_equal. extensionality s.
+        cbn in h. destruct h as [h1 h2].
+        rewrite -(H (get_heap s l) (h2 (get_heap s l))).
+        apply repr'_ext.
+        repeat f_equal.
+      - cbn. f_equal.
+        extensionality s.
+        f_equal.
+        extensionality s'.
+        destruct h as [h1 h2].
+        rewrite -(IHp h2).
+        apply repr'_ext.
+        reflexivity.
+      - cbn.
+        f_equal.
+        extensionality s.
+        simpl in h.
+        rewrite -(H s (h s)).
+        apply repr'_ext.
+        f_equal.
+    Qed.
+
 
     Let getLocations {I E} (P : package I E) : {fset Location} :=
       let '(locs; PP) := P in locs.
@@ -193,17 +230,17 @@ Module PackageRHL (π : RulesParam).
     Definition Pr_raw_program {L} {B}
                (p : raw_program B)
                (p_is_valid : valid_program L Game_import p)
-      : makeHeap_cT L -> SDistr (F_choice_prod_obj ⟨ B , makeHeap_cT L ⟩).
+      : heap_choiceType -> SDistr (F_choice_prod_obj ⟨ B , heap_choiceType ⟩).
     Proof.
       move => s0.
-      pose STDIST := thetaFstd B (FreeTranslate (exist _ p p_is_valid)) s0.
+      pose STDIST := thetaFstd B (repr (exist _ p p_is_valid)) s0.
       exact (STDIST prob_handler).
     Defined.
 
     Definition Pr_raw_func_program {L} {A} {B}
                (p : A -> raw_program B)
                (p_is_valid : forall a, valid_program L Game_import (p a))
-      : A -> makeHeap_cT L -> SDistr (F_choice_prod_obj ⟨ B , makeHeap_cT L ⟩).
+      : A -> heap_choiceType -> SDistr (F_choice_prod_obj ⟨ B , heap_choiceType ⟩).
     Proof.
       move => a s0.
       exact (Pr_raw_program (p a) (p_is_valid a) s0).
@@ -213,7 +250,7 @@ Module PackageRHL (π : RulesParam).
                (p : raw_package)
                (p_is_valid : valid_package L Game_import E p)
                (op : opsig) (Hin : op \in E) (arg : src op)
-      : makeHeap_cT L -> SDistr (F_choice_prod_obj ⟨ tgt op , makeHeap_cT L ⟩).
+      : heap_choiceType -> SDistr (F_choice_prod_obj ⟨ tgt op , heap_choiceType ⟩).
     Proof.
       move => s0.
       pose (get_raw_package_op p p_is_valid op Hin arg) as f.
@@ -222,7 +259,7 @@ Module PackageRHL (π : RulesParam).
 
     Definition Pr_op  {E : Interface} (P : package Game_import E)
                (op : opsig) (Hin : op \in E) (arg : src op)
-      : makeHeap_cT (getLocations P) -> SDistr (F_choice_prod_obj ⟨ tgt op , makeHeap_cT (getLocations P) ⟩).
+      : heap_choiceType -> SDistr (F_choice_prod_obj ⟨ tgt op , heap_choiceType ⟩).
     Proof.
       move => s0.
       destruct P as [L [PP PP_is_valid]].
@@ -264,54 +301,6 @@ Module PackageRHL (π : RulesParam).
       eapply hg.
     Defined.
 
-    (* Definition Pr (P : package Game_import A_export) : SDistr (bool_choiceType). *)
-    (* Proof. *)
-    (*   pose STDIST := thetaFstd _ (FreeTranslate (get_op P RUN RUN_in_A_export Datatypes.tt)). *)
-    (*   simpl in STDIST. *)
-    (*   pose SSDIST := STDIST prob_handler emptym. *)
-    (*   refine (SDistr_bind _ _ (fun '(b, _) => SDistr_unit _ b) SSDIST). *)
-    (* Defined. *)
-
-    Section semantic_judgement.
-      Context (locsl : {fset Location}).
-      Context (locsr : {fset Location}).
-      (* morphism *)
-      Let θ  := @thetaFstdex probE rel_choiceTypes chEmb (makeHeap_cT locsl) (makeHeap_cT locsr) prob_handler.
-      (* spec monad *)
-      Let WrelSt  := (rlmm_codomain θ).
-
-
-      Definition semantic_judgement (A1 A2 : ord_choiceType)
-                 (c1 : FrStP (makeHeap_cT locsl) A1) (c2 : FrStP (makeHeap_cT locsr) A2)
-                 (w  : Base.dfst (WrelSt ⟨ A1, A2 ⟩)) : Prop :=
-        (θ ⟨A1,A2⟩)∙1 ⟨c1,c2⟩ ≤ w.
-
-      Notation "⊨ c1 ≈ c2 [{ w }]" := (semantic_judgement _ _ c1 c2 w).
-
-      Definition fromPrePost {A1 A2 : ord_choiceType}
-                 (pre : (makeHeap_cT locsl * makeHeap_cT locsr) -> Prop)
-                 (post : (A1 * makeHeap_cT locsl) -> (A2 * makeHeap_cT locsr) -> Prop)
-        :  Base.dfst (WrelSt ⟨ A1, A2 ⟩).
-      Proof.
-        simpl.
-        unshelve econstructor.
-        - move=> [is1 is2]. unshelve econstructor.
-          + move=> myPost.
-             exact (  pre (is1,is2) /\
-                      forall as1 as2, (post as1 as2) -> myPost (as1, as2)).
-          + move => x y Hxy [H1 H2].
-            split.
-            * assumption.
-            * move => as1 as2 post12. apply: Hxy. by apply: H2.
-        - move => x y Heq π.
-          by rewrite Heq.
-      Defined.
-
-    End semantic_judgement.
-
-    Notation "⊨ ⦃ pre ⦄ c1 ≈ c2 ⦃ post ⦄" :=
-      (semantic_judgement _ _ _ _ c1 c2 (@fromPrePost _ _ _ _ pre post)).
-
     Import Num.Theory.
     Open Scope ring_scope.
     Open Scope real_scope.
@@ -329,83 +318,205 @@ Module PackageRHL (π : RulesParam).
     Notation "ϵ( GP )" := (fun A => AdvantageE (GP false) (GP true) A) (at level 90).
     Notation " G0 ≈[ R ] G1 " := (AdvantageE G0 G1 = R) (at level 50).
 
-    Ltac fold_FreeTranslate :=
-      change (FreeTranslate' ?p ?h) with (FreeTranslate (exist _ p h)).
-
-    Lemma some_lemma_for_prove_relational {export : Interface} {B}
-               (P1 : package Game_import export)
-               (P2 : package Game_import export)
-               (I : makeHeap_cT (getLocations P1) * makeHeap_cT (getLocations P2) -> Prop)
+    Lemma some_lemma_for_prove_relational {export : Interface} {B} {L1 L2 LA}
+               (P1 : opackage L1 Game_import export)
+               (P2 : opackage L2 Game_import export)
+               (I : heap_choiceType * heap_choiceType -> Prop)
                (Hempty : I (emptym, emptym))
                (H : forall (op : opsig) (Hin : op \in export) (arg : src op),
                    ⊨ ⦃ fun '(s1, s2) => I (s1, s2) ⦄
-                     (FreeTranslate (get_package_op P1 op Hin arg))
+                     (repr (get_opackage_op P1 op Hin arg))
                      ≈
-                     (FreeTranslate (get_package_op P2 op Hin arg))
+                     (repr (get_opackage_op P2 op Hin arg))
                      ⦃ fun '(b1, s1) '(b2, s2) => I (s1, s2) /\ b1 = b2 ⦄)
-               (A : raw_program B)
-               (A_is_valid : valid_program fset0 export A)
-               (s1 : makeHeap_cT (P1.π1)) (s2 : makeHeap_cT (P2.π1)) (Hs1s2 : I (s1, s2))
-      : dmargin fst (Pr_raw_program (raw_program_link A (P1.π2 ∙1))
-                                    (raw_program_link_valid _ _ _ _ _ _ (valid_injectLocations _ fset0 P1.π1 A (fsub0set P1.π1) A_is_valid) (P1.π2 ∙2)) s1) =
-        dmargin fst (Pr_raw_program (raw_program_link A (P2.π2 ∙1))
-                                    (raw_program_link_valid _ _ _ _ _ _ (valid_injectLocations _ fset0 P2.π1 A (fsub0set P2.π1) A_is_valid) (P2.π2 ∙2)) s2).
-      (* ER: for the proof we should have extra information about the second
-         component (preserves I), but let's see how the thing behaves so far *)
+               (A : program LA export B)
+               (s1 : heap_choiceType) (s2 : heap_choiceType) (Hs1s2 : I (s1, s2))
+      :
+        ⊨ ⦃ fun '(s1, s2) => I (s1, s2)  ⦄
+          repr (program_link (injectLocations (fsubsetUl LA (L1 :|: L2)) A) (opackage_inject_locations (fsubset_trans (fsubsetUl L1 L2) (fsubsetUr LA (L1 :|: L2))) P1))
+          ≈
+          repr (program_link (injectLocations (fsubsetUl LA (L1 :|: L2)) A) (opackage_inject_locations (fsubset_trans (fsubsetUr L1 L2) (fsubsetUr LA (L1 :|: L2))) P2))
+          ⦃ fun '(b1, s1) '(b2, s2) => b1 = b2 /\ I (s1, s2) ⦄.
     Proof.
-      destruct P1 as [L1 [P1a P1b]].
-      destruct P2 as [L2 [P2a P2b]].
+      destruct P1 as [P1a P1b].
+      destruct P2 as [P2a P2b].
+      destruct A as [A hA].
       induction A; intros.
-      - cbn. unfold SubDistr.SDistr_obligation_2.
-        rewrite !SDistr_rightneutral.
-        apply distr_ext. move => x0.
-        rewrite !dlet_unit. reflexivity.
-      - cbn. unfold SubDistr.SDistr_obligation_2.
-        rewrite !SDistr_assoc. admit.
-      - unfold Pr_raw_program.
-        cbn - [thetaFstd]. fold_FreeTranslate.
-        (* TW: I think this is much better now. *)
-        (* ER: this is nice, I would like to step a bit with raw_program_link and
-               FreeTranslate *)
-        simpl.
-        (* TW: Now it gets big because of thetaFstd *)
+      - cbn - [semantic_judgement].
+        unfold repr'_obligation_1.
+        eapply weaken_rule.
+        + apply ret_rule.
+        + cbv. intuition.
+      - destruct (lookup_op P1a o) eqn:lookup_op1.
+        2: { pose (P1b o) as Hbot. destruct hA as [hA1 hA2].
+             specialize (Hbot hA1). admit. }
+        cbn - [semantic_judgement].
+        fold_repr.
         admit.
-      - unfold Pr_raw_program.
-        simpl (FreeTranslate ⦑ raw_program_link (_putr l v A) ((L1; ⦑ P1a ⦒).π2) ∙1 ⦒).
-        (* PGH: the next two commands break compilation; commented out for now *)
-        (* simpl (thetaFstd B (ropr _ _ _ _ _)). *)
-        (* destruct (raw_program_link_valid B L1 export Game_import *)
-        (*                  (_putr l v A) P1a *)
-        (*                  (valid_injectLocations B fset0 L1 (_putr l v A) *)
-        (*                                         (fsub0set (T:=nat_ordType) L1) A_is_valid) P1b). *)
+      - unfold program_link. unfold injectLocations. unfold opackage_inject_locations.
+        simpl (raw_program_link _). unfold "∙1".
+         match goal with
+        | |- ⊨ ⦃ _ ⦄ repr ⦑ _getr ?l ?k ⦒ ≈ _ ⦃ _ ⦄ =>
+          eassert (⦑ _getr l k ⦒ =
+                   bind _ _ ⦑ _getr l (fun x : Value => _ret x) ⦒ (fun v => ⦑ k v ⦒)) as Hl
+        end.
+        { apply program_ext. cbn. reflexivity. }
+        rewrite Hl.
+        rewrite repr_bind.
+        match goal with
+        | |- ⊨ ⦃ _ ⦄ _ ≈ repr ⦑ _getr ?l ?k ⦒ ⦃ _ ⦄ =>
+          eassert (⦑ _getr l k ⦒ =
+                   bind _ _ ⦑ _getr l (fun x : Value => _ret x) ⦒ (fun v => ⦑ k v ⦒)) as Hr
+        end.
+        { apply program_ext. cbn. reflexivity. }
+        rewrite Hr.
+        rewrite repr_bind.
+        eapply weaken_rule.
+        + eapply bind_rule.
+          ++ admit.
+          ++ intros a1 a2. admit.
+        + admit.
+      - admit.
+      - unfold program_link. unfold injectLocations. unfold opackage_inject_locations.
+        simpl (raw_program_link _). unfold "∙1".
+         match goal with
+        | |- ⊨ ⦃ _ ⦄ repr ⦑ _sampler ?l ?k ⦒ ≈ _ ⦃ _ ⦄ =>
+          eassert (⦑ _sampler l k ⦒ =
+                   bind _ _ ⦑ _sampler l (fun x : Arit l => _ret x) ⦒ (fun v => ⦑ k v ⦒)) as Hl
+        end.
+        { apply program_ext. cbn. reflexivity. }
+        rewrite Hl.
+        rewrite repr_bind.
+        match goal with
+        | |- ⊨ ⦃ _ ⦄ _ ≈ repr ⦑ _sampler ?l ?k ⦒ ⦃ _ ⦄ =>
+          eassert (⦑ _sampler l k ⦒ =
+                   bind _ _ ⦑ _sampler l (fun x : Arit l => _ret x) ⦒ (fun v => ⦑ k v ⦒)) as Hr
+        end.
+        { apply program_ext. cbn. reflexivity. }
+        rewrite Hr.
+        rewrite repr_bind.
+
         admit.
-      - unfold Pr_raw_program in *.
-        simpl (FreeTranslate _).
-        simpl (thetaFstd).
     Admitted.
+
+    Lemma get_raw_package_op_link {L} {I E} {o : opsig}
+          (hin : o \in E) (arg : src o) (p1 p2 : raw_package)
+          (hp1 : valid_package L I E p1)
+          (hpl : valid_package L I E (raw_link p1 p2))
+          : (get_raw_package_op (raw_link p1 p2) hpl o hin arg) ∙1 =
+            raw_program_link ((get_raw_package_op p1 hp1 o hin arg) ∙1) p2.
+    Proof.
+      admit.
+    Admitted.
+
+
 
     (* ER: How do we connect the package theory with the RHL?
            Something along the following lines should hold? *)
-    Definition prove_relational {export : Interface}
-               (P1 : package Game_import export)
-               (P2 : package Game_import export)
-               (I : makeHeap_cT (getLocations P1) * makeHeap_cT (getLocations P2) -> Prop)
+    Definition prove_relational {export : Interface} {L1 L2}
+               (P1 : opackage L1 Game_import export)
+               (P2 : opackage L2 Game_import export)
+               (I : heap_choiceType * heap_choiceType -> Prop)
                (Hempty : I (emptym, emptym))
                (H : forall (op : opsig) (Hin : op \in export) (arg : src op),
                    ⊨ ⦃ fun '(s1, s2) => I (s1, s2) ⦄
-                     (FreeTranslate (get_op P1 op Hin arg))
+                     (repr (get_opackage_op P1 op Hin arg))
                      ≈
-                     (FreeTranslate (get_op P2 op Hin arg))
+                     (repr (get_opackage_op P2 op Hin arg))
                      ⦃ fun '(b1, s1) '(b2, s2) => I (s1, s2) /\ b1 = b2  ⦄)
-      : P1 ≈[ fun A => 0 ] P2.
+      : (L1; P1) ≈[ fun A => 0 ] (L2; P2).
     Proof.
-      destruct P1 as [locs1 pp1].
-      destruct P2 as [locs2 pp2].
-      unfold getLocations in I, H.
       extensionality A.
-      unfold semantic_judgement in H.
+      unfold Adversary4Game in A.
       unfold AdvantageE, Pr.
-      admit.
+      pose r' := get_package_op A RUN RUN_in_A_export.
+      pose r := r' tt.
+      pose Hlemma := (some_lemma_for_prove_relational _ _ _ Hempty H r emptym emptym Hempty).
+      assert (∀ x y : tgt RUN * heap_choiceType,
+                 (let '(b1, s1) := x in λ '(b2, s2), b1 = b2 s/\ I (s1, s2)) y → (fst x == true) ↔ (fst y == true)) as Ha.
+      { intros [b1 s1] [b2 s2]. simpl.
+        intros [H1 H2]. rewrite H1. intuition. }
+      pose Heq := (Pr_eq _ _ _ _ Hlemma Hempty Ha).
+      simpl in Heq.
+      simpl in Hlemma.
+      unfold θ_dens in Heq.
+      simpl in Heq. unfold pr in Heq.
+      simpl in Heq.
+      unfold Pr_op.
+      pose _rhs := (thetaFstd _ (repr (program_link
+            (injectLocations (fsubsetUl (T:=nat_ordType) (getLocations A) (L1 :|: L2)) r)
+            (opackage_inject_locations
+               (fsubset_trans (T:=nat_ordType) (y:=L1 :|: L2) (x:=L1)
+                  (z:=getLocations A :|: (L1 :|: L2)) (fsubsetUl (T:=nat_ordType) L1 L2)
+                  (fsubsetUr (T:=nat_ordType) (getLocations A) (L1 :|: L2))) P1))) emptym).
+      pose rhs := _rhs prob_handler.
+      simpl in _rhs, rhs.
+      pose lhs := (let (L, o) := link A (L1; P1) in
+                   let (PP, PP_is_valid) := o in
+                   Pr_raw_package_op PP PP_is_valid RUN RUN_in_A_export tt emptym).
+      assert (lhs = rhs).
+      { unfold lhs, rhs, _rhs. simpl.
+        unfold Pr_raw_package_op. unfold Pr_raw_program.
+        unfold thetaFstd. simpl. apply f_equal2. 2: { reflexivity. }
+        apply f_equal. apply f_equal.
+        unfold getLocations. unfold ".π1".
+        destruct A as [LA [A A_valid]].
+        apply repr'_ext.
+        erewrite (get_raw_package_op_link RUN_in_A_export tt (trim A_export ((LA; ⦑ A ⦒).π2) ∙1) (P1 ∙1) _ _).
+        apply f_equal2. 2: { reflexivity. }
+                                                                                                              admit.
+      }
+      unfold lhs in H0.
+      rewrite H0.
+
+      pose _rhs' := (thetaFstd _ (repr (program_link
+            (injectLocations (fsubsetUl (T:=nat_ordType) (getLocations A) (L1 :|: L2)) r)
+            (opackage_inject_locations
+               (fsubset_trans (T:=nat_ordType) (y:=L1 :|: L2) (x:=L2)
+                  (z:=getLocations A :|: (L1 :|: L2)) (fsubsetUr (T:=nat_ordType) L1 L2)
+                  (fsubsetUr (T:=nat_ordType) (getLocations A) (L1 :|: L2))) P2))) emptym).
+      pose rhs' := _rhs' prob_handler.
+      simpl in _rhs', rhs'.
+      pose lhs' := (let (L, o) := link A (L2; P2) in
+                   let (PP, PP_is_valid) := o in
+                   Pr_raw_package_op PP PP_is_valid RUN RUN_in_A_export tt emptym).
+      assert (lhs' = rhs') as H0'.
+      { unfold lhs', rhs', _rhs'. simpl.
+        unfold Pr_raw_package_op. unfold Pr_raw_program.
+        unfold thetaFstd. simpl. apply f_equal2. 2: { reflexivity. }
+        apply f_equal. apply f_equal.  admit. }
+      unfold lhs' in H0'.
+      rewrite H0'.
+      unfold rhs', _rhs', rhs, _rhs.
+
+      unfold SDistr_bind. unfold SDistr_unit.
+      simpl.
+      rewrite !dletE.
+      assert (forall x : bool_choiceType * heap_choiceType, ((let '(b, _) := x in dunit (R:=R) (T:=bool_choiceType) b) true) == (x.1 == true)%:R).
+      { intros [b s].
+        simpl. rewrite dunit1E. intuition. }
+      assert (forall y, (λ x : prod_choiceType (tgt RUN) heap_choiceType, (y x) * (let '(b, _) := x in dunit (R:=R) (T:=tgt RUN) b) true) = (λ x : prod_choiceType (tgt RUN) heap_choiceType, (x.1 == true)%:R * (y x))) as Hrew.
+      { intros y. extensionality x.
+        destruct x as [x1 x2].
+        rewrite dunit1E.
+        simpl. rewrite GRing.mulrC. reflexivity. }
+      rewrite !Hrew.
+      unfold TransformingLaxMorph.rlmm_from_lmla_obligation_1. simpl.
+      unfold SubDistr.SDistr_obligation_2. simpl.
+      unfold OrderEnrichedRelativeAdjunctionsExamples.ToTheS_obligation_1. simpl.
+      rewrite !SDistr_rightneutral. simpl.
+      rewrite Heq.
+      rewrite /StateTransfThetaDens.unaryStateBeta'_obligation_1.
+      unfold TransformingLaxMorph.rlmm_from_lmla_obligation_1, stT_thetaDens_adj.
+      assert (forall (x : R), `|x - x| = 0) as Hzero.
+      { intros x.
+        assert (x - x = 0) as H3.
+        { apply /eqP. rewrite GRing.subr_eq0. intuition.  }
+        rewrite H3. apply mc_1_10.Num.Theory.normr0.
+        }
+      rewrite Hzero.
+      reflexivity.
+      Unshelve.
     Admitted.
   End Games.
 
